Start of the program for dirtree2mem.
New security proofs (or impossibility of them) for basic instructions.

src/BasicSecurity2.v
@@ -18,8 +18,18 @@ Require Import Array.
 Require Import Bytes.
 Require Import Mem.
 Require Import Cache. 
+Require Import GenSepN.
+Require Import ClassicalFacts.
 
 Set Implicit Arguments.
+
+
+  Ltac sub_inv := 
+  match goal with
+  | [H: ?a = _, H0: ?a = _ |- _ ] => rewrite H in H0; inversion H0; subst; eauto
+  end.
+Ltac sep_unfold H := unfold sep_star in H; rewrite sep_star_is in H; unfold sep_star_impl in H; repeat deex.
+
 
 (** * Some helpful [prog] combinators and proofs *)
 
@@ -33,30 +43,34 @@ Qed.
 
 Hint Resolve sync_invariant_possible_sync.
 
-Definition pred_upd_w (pre: pred) (a: addr) (v: valu) : pred :=
-  fun (m: @mem _ addr_eq_dec valuset) => 
-    match m a with
-    | None => False
-    | Some vs => let (v', ovs) := vs in
-                          match ovs with
-                          | nil => False
-                          | h :: t => v = v' /\ pre (upd m a (h, t))
-                          end
-    end.                  
+(* 
+    Meaning of the definition:
+      Take two memories 
+          m1 = x \union mp
+          m2 = y \union mp
+      Assume: 
+          F1 x
+          F2 y
+          pre mp
+          If p executes with m1 vm hm, then produces out1
+       Then:
+          there exists two memories such that
+              m1' = x' \union mr
+              m2' = y' \union mr
+          memories are m1'(m2') vm' hm' after executing p on m1(m2)
+          output of both executions is r
+          post mr
+        OR
+          "same for crash"
+*)
+(* Frames does not say for the remainder memory is unchanged or not. *)
+(* 
+    Can we say
+      Defintion pequal P Q := forall m, P m <-> Q m.
+      Lemma exists_diskIs: forall F, exists p m, F m -> pequal F ([[ P ]] * diskIs m).
+*)
 
-Lemma definition_is_ok: forall pre a v vs m,
-m a = Some vs -> pre m <-> pred_upd_w pre a v (upd m a (v, vsmerge vs)).
-Proof.
-    unfold pred_upd_w; simpl; intros.
-    - unfold vsmerge; destruct vs; simpl.
-    rewrite upd_eq; auto.
-    rewrite upd_repeat.
-    rewrite upd_nop; auto.
-    split; intros; auto.
-    destruct H0; auto.
-Qed.
-
-Definition prog_secure T (p : prog T) (pre : pred) (post : pred):=
+Definition prog_secure T (p : prog T) (pre : pred) (post : pred) :=
   forall m1 m2 mp F1 F2 out1 vm hm,
 
   (F1 * diskIs mp)%pred m1 ->
@@ -76,6 +90,507 @@ Definition prog_secure T (p : prog T) (pre : pred) (post : pred):=
    exec m2 vm hm p (Crashed _ m2' hm') /\
    (F1 * diskIs mc)%pred m1' /\
    (F2 * diskIs mc)%pred m2').
+
+Theorem bind_secure:
+  forall T1 T2 (p1 : prog T1) (p2 : T1 -> prog T2) pre post1 post2,
+  prog_secure p1 pre post1 ->
+  (forall x, prog_secure (p2 x) post1 post2) ->
+  prog_secure (Bind p1 p2) pre post2.
+Proof.
+  unfold prog_secure; intros.
+  inv_exec.
+  - (* p1 Finished *)
+    specialize (H _ _ _ _ _ _ _ _ H1 H2 H3 H11).
+    intuition; repeat deex; try congruence.
+    inversion H4; subst.
+    specialize (H0 r _ _ _ _ _ _ _ _ H5 H6 H8 H14).
+    intuition; repeat deex.
+    + left.
+      do 6 eexists; intuition eauto.
+    + right.
+      do 4 eexists; intuition eauto.
+  - (* p1 Failed *)
+    specialize (H _ _ _ _ _ _ _ _ H1 H2 H3 H10).
+    intuition; repeat deex; try congruence.
+  - (* p1 Crashed *)
+    specialize (H _ _ _ _ _ _ _ _ H1 H2 H3 H10).
+    intuition; repeat deex; try congruence.
+    right.
+    inversion H4; subst.
+    do 4 eexists; intuition.
+    constructor.
+    eauto.
+    eauto.
+    eauto.
+Qed.
+
+Theorem bind_secure_weaker:
+  forall T1 T2 (p1 : prog T1) (p2 : T1 -> prog T2) pre post1 post2,
+  prog_secure p1 pre post1 ->
+  (forall m vm hm m' vm' hm' r, exec m vm hm p1 (Finished m' vm' hm' r) -> prog_secure (p2 r) post1 post2) ->
+  prog_secure (Bind p1 p2) pre post2.
+Proof.
+  unfold prog_secure; intros.
+  inv_exec.
+  - (* p1 Finished *)
+    specialize (H _ _ _ _ _ _ _ _ H1 H2 H3 H11).
+    intuition; repeat deex; try congruence.
+    inversion H4; subst.
+    specialize (H0 _ _ _ _ _ _ r H11 _ _ _ _ _ _ _ _ H5 H6 H8 H14).
+    intuition; repeat deex.
+    + left.
+      do 6 eexists; intuition eauto.
+    + right.
+      do 4 eexists; intuition eauto.
+  - (* p1 Failed *)
+    specialize (H _ _ _ _ _ _ _ _ H1 H2 H3 H10).
+    intuition; repeat deex; try congruence.
+  - (* p1 Crashed *)
+    specialize (H _ _ _ _ _ _ _ _ H1 H2 H3 H10).
+    intuition; repeat deex; try congruence.
+    right.
+    inversion H4; subst.
+    do 4 eexists; intuition.
+    constructor.
+    eauto.
+    eauto.
+    eauto.
+Qed.
+
+Lemma mem_disjoint_sync_mem_l:
+  forall AT AEQ (m1 m2: @mem AT AEQ _),
+  mem_disjoint m1 m2
+  -> mem_disjoint (sync_mem m1) m2.
+Proof.
+  unfold mem_disjoint, sync_mem in *; intuition.
+  apply H.
+  repeat deex.
+  exists a.
+  destruct (m1 a); try congruence.
+  destruct (m2 a); try congruence.
+  eauto.
+Qed.
+
+Lemma exec_mem_disjoint:
+  forall T (p: prog T) m1 m2 m3 vm hm  vm' hm' r,
+  mem_disjoint m1 m2
+  -> exec m1 vm hm p (Finished m3 vm' hm' r)
+  -> mem_disjoint m3 m2.
+Proof.
+  induction p; intros; inv_exec; auto.
+  eapply mem_disjoint_upd; eauto.
+  apply mem_disjoint_sync_mem_l; auto.
+  eapply mem_disjoint_upd; eauto.
+  eapply H; [ | eauto].
+  eapply IHp; eauto.
+Qed.
+
+Lemma diskIs_id: forall AT AEQ V (m:Mem.mem), @diskIs AT AEQ V m m.
+Proof. intros; unfold diskIs; reflexivity. Qed.
+
+Hint Resolve diskIs_id.
+
+Lemma diskIs_mem_disjoint :
+  forall AT AEQ V (m m1 m2: @mem AT AEQ V),
+  (diskIs m1 ✶ diskIs m2)%pred m
+  -> mem_disjoint m1 m2.
+Proof.
+  intros.
+  unfold sep_star in H; rewrite sep_star_is in H; unfold sep_star_impl in H.
+  repeat deex.
+  destruct H1; destruct H3; subst; auto.
+Qed.
+
+Lemma mem_union_disjoint_sel:
+  forall AT AEQ V (m1 m2: @mem AT AEQ V) a v,
+  mem_disjoint m1 m2 ->
+  m1 a = Some v ->
+  mem_union m1 m2 a = m1 a.
+Proof.
+ intros. 
+ apply mem_union_sel_l; auto.
+ eapply mem_disjoint_either; eauto.
+Qed.
+
+(* Failed attempt 1 *)
+Module Failed1.
+
+Definition prog_secure' T (p : prog T) (pre post: @pred _ addr_eq_dec _) :=
+  forall m mp F vm hm,
+  (F * diskIs mp)%pred m ->
+  pre mp ->
+  (exists r vm' hm' mr, exec mp vm hm p (Finished mr vm' hm' r) /\ post mr)
+  \/ exists hm' mc, exec mp vm hm p (Crashed _ mc hm').
+  
+Theorem bind_secure':
+  forall T1 T2 (p1 : prog T1) (p2 : T1 -> prog T2) pre post1 post2,
+  prog_secure' p1 pre post1 ->
+  (forall x, prog_secure' (p2 x) post1 post2) ->
+  prog_secure' (Bind p1 p2) pre post2.
+Proof.
+  unfold prog_secure'; intros.
+  specialize (H _ _ _ vm hm H1 H2).
+  destruct H;  repeat deex.
+  eapply diskIs_sep_star_split in H1; repeat deex.
+  inversion H; subst.
+  specialize (H0 r (mem_union mp0 mr) mr F vm' hm').
+  destruct H0; eauto.
+  apply sep_star_mem_union; auto.
+  apply mem_disjoint_comm; eapply exec_mem_disjoint; eauto.
+  assert (A: diskIs m m).
+  apply diskIs_id.
+  apply H6 in A.
+  apply mem_disjoint_comm; eapply diskIs_mem_disjoint; eauto.
+  repeat deex.
+  left; repeat eexists; eauto.
+  repeat deex.
+  right; repeat eexists; eauto.
+  right; repeat eexists; eauto.
+Qed.
+
+Theorem bind_secure'_rev_l:
+  forall T1 T2 (p1 : prog T1) (p2 : T1 -> prog T2) pre post,
+  T2 
+  -> EqDec T2
+  -> prog_secure' (Bind p1 p2) pre post
+  -> exists post1, prog_secure' p1 pre post1.
+Proof.
+  unfold prog_secure'; intros; eexists; intros. 
+  - specialize (H _ _ _ vm hm H0 H1).
+    destruct H; repeat deex.
+    * inv_exec.
+      left; repeat eexists; eauto.
+      apply diskIs_id.
+    * inv_exec.
+      left; repeat eexists; eauto.
+      right; repeat eexists; eauto.
+  Unshelve.
+  all: trivial.
+  repeat constructor; auto.
+Qed.
+
+
+Lemma exec_sep_star:
+  forall T (p: prog T) m1 m1' m2 vm vm' hm hm' r,
+  mem_disjoint m1 m2
+  -> exec m1 vm hm p (Finished m1' vm' hm' r)
+  -> exec (mem_union m1 m2) vm hm p (Finished (mem_union m1' m2) vm' hm' r).
+Proof.
+  induction p; intros; inv_exec; try solve [repeat econstructor; eauto].
+  - repeat econstructor.
+     apply mem_union_addr; eauto.
+  - rewrite mem_union_upd.
+    repeat econstructor.
+    apply mem_union_addr; eauto.
+  - admit. (* Sync *)
+  - rewrite mem_union_upd.
+    repeat econstructor.
+    apply mem_union_addr; eauto.
+  - inversion H8; eauto.
+  - inversion H14; eauto. 
+  - eapply  XBindFinish.
+    eapply IHp; eauto.
+    eapply H; eauto.
+    eapply exec_mem_disjoint; eauto.
+Abort.
+
+Lemma exec_eq:
+  forall T (p: prog T) m vm hm m1' vm1' hm1' r1 m2' vm2' hm2' r2,
+  exec m vm hm p (Finished m1' vm1' hm1' r1)
+  ->  exec m vm hm p (Finished m2' vm2' hm2' r2)
+  -> m1' = m2' /\ vm1' = vm2' /\ hm1' = hm2' /\ r1 = r2.
+Proof.
+  induction p; intros; try solve [inv_exec; inv_exec; eauto; sub_inv].
+  - admit. (* Trim changes memory nondeterministically *)
+  - admit. (* VarAlloc changes vm and also returns nondeterministically *)
+  - admit. (* VarGet returns nondeterministically *)
+  - admit. (* Rdtsc returns nondeterministically *)
+  - inv_exec; inv_exec.
+    edestruct IHp with (m1':= m') (m2':= m'0); eauto.
+    destruct H1; subst.
+    destruct H2; subst.
+    eauto.
+Abort.
+
+Theorem prog_secure'_is_noninterference :
+  forall T (p : prog T) pre post a v1 v2 m1 m2 mp vm hm,
+  prog_secure' p pre post ->
+  (a |+> v1 * diskIs mp)%pred m1 ->
+  (a |+> v2 * diskIs mp)%pred m2 ->
+  pre mp ->
+  forall m1' vm' hm' v,
+  exec m1 vm hm p (Finished m1' vm' hm' v) ->
+  exists m2' vm'' hm'',
+  exec m2 vm hm p (Finished m2' vm'' hm'' v).
+Proof.
+  induction p; unfold prog_secure' in *; intros.
+  - specialize (H _ _ _ vm hm H0 H2) as Hx.
+     intuition; repeat deex; try congruence.
+     inv_exec; inv_exec.
+     repeat eexists; eauto.
+     inv_exec; inv_exec.
+  - specialize (H _ _ _ vm hm H0 H2) as Hx.
+     intuition; repeat deex; try congruence.
+     inv_exec; inv_exec.
+     admit. (*Solvable*)
+     inv_exec; inv_exec.
+     (*Not solvable! Definition is wrong!*)
+Abort.
+End Failed1.
+
+Module Variant2.
+Definition prog_secure' T (p : prog T) (pre : pred) (post : pred) :=
+  forall m1 m2 F1 F2 out1 vm hm,
+
+  (F1 * pre)%pred m1 ->
+  (F2 * pre)%pred m2 ->
+  exec m1 vm hm p out1 ->
+
+  (exists r m1' m2' vm' hm',
+   out1 = Finished m1' vm' hm' r /\
+   exec m2 vm hm p (Finished m2' vm' hm' r) /\
+   (F1 * post)%pred m1' /\
+   (F2 * post)%pred m2') \/
+
+  (exists m1' m2' hm' mc,
+   out1 = Crashed _ m1' hm' /\
+   exec m2 vm hm p (Crashed _ m2' hm') /\
+   (F1 * diskIs mc)%pred m1' /\
+   (F2 * diskIs mc)%pred m2').
+   
+Theorem prog_secure'_is_noninterference :
+  forall T (p : prog T) pre post a v1 v2 m1 m2 mp vm hm,
+  prog_secure' p pre post ->
+  (a |+> v1 * diskIs mp)%pred m1 ->
+  (a |+> v2 * diskIs mp)%pred m2 ->
+  pre mp ->
+  forall m1' vm' hm' v,
+  exec m1 vm hm p (Finished m1' vm' hm' v) ->
+  exists m2' vm'' hm'',
+  exec m2 vm hm p (Finished m2' vm'' hm'' v).
+Proof.
+  unfold prog_secure'; intros.
+  erewrite diskIs_pred in H0; eauto.
+  erewrite diskIs_pred in H1; eauto.
+  specialize (H _ _ _ _ _ _ _ H0 H1 H3).
+  intuition; repeat deex; try congruence.
+  do 3 eexists.
+  inversion H4; subst.
+  eauto.
+Qed.
+
+Theorem sync_secure':
+  prog_secure' Sync (fun m => forall a, exists vs, m a = Some vs) (fun m => forall a, exists v, m a = Some (v, nil)).
+Proof.
+  unfold prog_secure'; intros.
+  inv_exec.
+  specialize (H _ _ _ vm hm H1 H2).
+  destruct H;  repeat deex.
+  eapply diskIs_sep_star_split in H1; repeat deex.
+  inversion H; subst.
+  specialize (H0 r (mem_union mp0 mr) mr F vm' hm').
+  destruct H0; eauto.
+  apply sep_star_mem_union; auto.
+  apply mem_disjoint_comm; eapply exec_mem_disjoint; eauto.
+  assert (A: diskIs m m).
+  apply diskIs_id.
+  apply H6 in A.
+  apply mem_disjoint_comm; eapply diskIs_mem_disjoint; eauto.
+  repeat deex.
+  left; repeat eexists; eauto.
+  repeat deex.
+  right; repeat eexists; eauto.
+  right; repeat eexists; eauto.
+Qed.
+
+Lemma prog_secure_eq:
+  forall T (p: prog T) pre post,
+  prog_secure' p pre post ->
+  prog_secure p pre post.
+Proof.
+  unfold prog_secure, prog_secure'; intros.
+  erewrite diskIs_pred in H0; eauto.
+  erewrite diskIs_pred in H1; eauto.
+  specialize (H _ _ _ _ _ _ _ H0 H1 H3).
+  intuition; repeat deex; try congruence.
+  sep_unfold H5.
+  sep_unfold H7.
+  left; repeat eexists; eauto.
+  (* Memory contents can be different *)
+Abort.
+End Variant2.
+
+Definition valu0 n := bytes2valu  (natToWord (valubytes*8) n).
+Definition valuset0 n := (valu0 n, valu0 (S n)::nil).
+
+Theorem sync_not_secure:
+  forall pre post,
+  (exists m, pre m /\ exists a, m a = None) ->
+  ~ prog_secure Sync pre post.
+Proof.
+  unfold prog_secure, not; intros.
+  repeat deex.
+  remember (insert (@empty_mem _ addr_eq_dec _) a (valuset0 0)) as mx.
+ remember (insert (@empty_mem _ addr_eq_dec _) a (valuset0 1)) as my.
+  edestruct H0; eauto.
+  - instantiate (1:= mem_union mx m).
+    instantiate (1:= diskIs mx).
+    apply sep_star_mem_union; auto.
+    unfold mem_disjoint, not; intros; repeat deex.
+    unfold insert, empty_mem in H3.
+    destruct (addr_eq_dec a0 a); subst; try sub_inv.
+    inversion H3.
+  
+  - instantiate (1:= mem_union my m).
+    instantiate (1:= diskIs my).
+    apply sep_star_mem_union; auto.
+    unfold mem_disjoint, not; intros; repeat deex.
+    unfold insert, empty_mem in H3.
+    destruct (addr_eq_dec a0 a); subst; try sub_inv.
+    inversion H3.
+    
+  - repeat deex.
+    inversion H3; subst; clear H3.
+    inv_exec.
+    sep_unfold H4.
+    inversion H4; inversion H8; subst; clear H4 H8.
+    assert (A: (mem_union (insert empty_mem a (valuset0 0)) m2) a = Some (valuset0 0)).
+    unfold mem_union; simpl.
+    unfold insert, empty_mem; simpl.
+    destruct (addr_eq_dec a a); try omega; auto.
+    rewrite <- H3 in A.
+    unfold sync_mem, mem_union, insert, empty_mem, valuset0 in A; simpl in A.
+    destruct (addr_eq_dec a a); try omega; auto.
+    inversion A.
+    
+  - repeat deex.
+    inversion H3.
+    
+  Unshelve.
+  all: repeat econstructor; eauto.
+Qed.
+
+
+Theorem trim_secure:
+  forall a vs,
+  prog_secure (Trim a) (a|->vs)%pred (a|->?)%pred.
+Proof.
+  unfold prog_secure; intros.
+  inv_exec.
+  - left. 
+    do 6 eexists; repeat split.
+    + econstructor.
+      econstructor.
+      rewrite (diskIs_pred _ H1) in H0.
+      eapply ptsto_valid' in H0; eauto.
+    + eapply diskIs_sep_star_upd. 2: eauto.
+      unfold ptsto in H1; intuition eauto.
+    + eapply diskIs_sep_star_upd. 2: eauto.
+      unfold ptsto in H1; intuition eauto.
+    + eapply pimpl_apply.
+      2: eapply ptsto_upd.
+      2: pred_apply; cancel.
+      cancel.
+  - exfalso.
+    rewrite (diskIs_pred _ H1) in H.
+    eapply ptsto_valid' in H.
+    congruence.
+Qed.
+
+Theorem varalloc_secure:
+  forall T (a: T),
+  prog_secure (VarAlloc a) emp emp.
+Proof.
+  unfold prog_secure; intros.
+  apply emp_empty_mem_only in H1; subst.
+  inv_exec.
+  left; repeat eexists; eauto.
+Qed.
+
+Theorem vardelete_secure:
+  forall i,
+  prog_secure (VarDelete i) emp emp.
+Proof.
+  unfold prog_secure; intros.
+  apply emp_empty_mem_only in H1; subst.
+  inv_exec.
+  - left; repeat eexists; eauto.
+  - inversion H8; subst.
+     (* Fail Case not possible to prove *)
+Abort.
+
+
+Theorem varget_secure:
+  forall T i,
+  prog_secure (@VarGet T i) emp emp.
+Proof.
+  unfold prog_secure; intros.
+  apply emp_empty_mem_only in H1; subst.
+  inv_exec.
+  - left; repeat eexists; eauto.
+  - inversion H8; subst.
+    sub_inv.
+     (* Fail Case not possible to prove *)
+Abort.
+
+
+
+Theorem varget_secure:
+  forall T i (v: T),
+  prog_secure (VarSet i v) emp emp.
+Proof.
+  unfold prog_secure; intros.
+  apply emp_empty_mem_only in H1; subst.
+  inv_exec.
+  - left; repeat eexists; eauto.
+  - (* Fail Case not possible to prove *)
+Abort.
+
+
+Theorem debug_secure:
+  forall s a,
+  prog_secure (Debug s a) emp emp.
+Proof.
+  unfold prog_secure; intros.
+  apply emp_empty_mem_only in H1; subst.
+  inv_exec.
+  left; repeat eexists; eauto.
+Qed.
+
+Theorem rdtsc_secure:
+  prog_secure (Rdtsc) emp emp.
+Proof.
+  unfold prog_secure; intros.
+  apply emp_empty_mem_only in H1; subst.
+  inv_exec.
+  left; repeat eexists; eauto.
+Qed.
+
+
+Theorem hash_secure:
+  forall sz buf,
+  prog_secure (@Hash sz buf) emp emp.
+Proof.
+  unfold prog_secure; intros.
+  apply emp_empty_mem_only in H1; subst.
+  inv_exec.
+  left; repeat eexists; eauto.
+Qed.
+
+Theorem hash2_secure:
+  forall sz1 sz2 buf1 buf2,
+  prog_secure (@Hash2 sz1 sz2 buf1 buf2) emp emp.
+Proof.
+  unfold prog_secure; intros.
+  apply emp_empty_mem_only in H1; subst.
+  inv_exec.
+  left; repeat eexists; eauto.
+Qed.
+
+
+
+
+
 
 Definition addr_is_in {AT AEQ V} (a: AT) (pre: pred):=
   forall (m: @mem AT AEQ V), pre m -> indomain a m.  
@@ -133,16 +648,7 @@ Proof.
     deex; eexists; eauto.
 Qed.
 
-Lemma mem_union_disjoint_sel:
-  forall AT AEQ V (m1 m2: @mem AT AEQ V) a v,
-  mem_disjoint m1 m2 ->
-  m1 a = Some v ->
-  mem_union m1 m2 a = m1 a.
-Proof.
- intros. 
- apply mem_union_sel_l; auto.
- eapply mem_disjoint_either; eauto.
-Qed.
+
        
 
 
@@ -525,71 +1031,78 @@ Proof.
 Qed.
 End V2.
 
-Module TwoLevel.
-Module L1.
 
+
+Inductive prog_secure_strict: forall T AT AEQ V, prog T -> @pred AT AEQ V -> @pred AT AEQ V -> Prop :=
+| PSRet : forall T AT AEQ V (v: T), 
+      @prog_secure_strict T AT AEQ V (Ret v) emp emp
+| PSRead : forall V a (vs: V),
+      @prog_secure_strict _ _ addr_eq_dec _ (Read a) (a|->vs) (a|->vs)
+| PSWrite : forall a v vs,
+      @prog_secure_strict _ _ addr_eq_dec _ (Write a v) (a |-> vs)%pred (a |-> (v, vsmerge vs))%pred
+| PSBind : forall AT AEQ V T1 T2 (p1 : prog T1) (p2 : T1 -> prog T2) (pre post1 post2: @pred AT AEQ V),
+      prog_secure_strict p1 pre post1 ->
+      (forall x, prog_secure_strict (p2 x) post1 post2) ->
+      prog_secure_strict (Bind p1 p2) pre post2
+| PSImpl : forall T AT AEQ V (p : prog T) (pre pre' post post': @pred AT AEQ V),
+      pre' =p=> pre ->
+      post =p=> post' ->
+      prog_secure_strict p pre post ->
+      prog_secure_strict p pre' post'
+| PSFrame : forall T AT AEQ V (p : prog T) (pre post F: @pred AT AEQ V),
+  prog_secure_strict p pre post ->
+  prog_secure_strict p (F * pre)%pred (F * post)%pred.
+
+Hint Constructors prog_secure_strict.
+
+
+
+Module TwoLevel.
+
+Module L1.
   (* Memory represented as an array of indices *)
-  
   Record array_rep := {
-    Log : list valuset;
     Data : list valuset
   }.
   
-  Definition rep (arr: array_rep) : @pred addr addr_eq_dec _ :=
-    (arrayN (@ptsto addr _ _) 0 (Log arr) * arrayN (@ptsto addr _ _) (length (Log arr)) (Data arr))%pred.
-
-  Definition read_log arr i def:=
-    if lt_dec i (length (Log arr)) then
-      v <- Read i; Ret v
-    else
-      Ret def.
-
-  Definition write_log arr i v def:=
-    if lt_dec i (length (Log arr)) then
-      _ <- Write i v; 
-      let vs := selN (Log arr) i def in
-      Ret ({| Log:= updN (Log arr) i (v, vsmerge vs); Data:= (Data arr) |})
-    else
-      Ret arr.
+  Definition rep (arr: array_rep) : @pred addr addr_eq_dec _ := 
+      arrayN (@ptsto addr _ _) 0 (Data arr).
   
   Definition read_data arr i def:=
     if lt_dec i (length (Data arr)) then
-      v <- Read (i + (length (Log arr))); Ret v
+      v <- Read i; Ret v
     else
       Ret def.
 
   Definition write_data arr i v def:=
     if lt_dec i (length (Data arr)) then
-      _ <- Write (i + (length (Log arr))) v; 
+      _ <- Write i v; 
       let vs := selN (Data arr) i def in
-      Ret ({| Log:= Log arr; Data:= updN (Data arr) i (v, vsmerge vs) |})
+      Ret ({| Data:= updN (Data arr) i (v, vsmerge vs) |})
     else
       Ret arr.
-
 End L1.
 
 Module L2.
 Import L1.
 
   Variable file_size: nat. 
+  Hypothesis file_size_nonzero: file_size <> 0.
   Record file := { 
-     Meta: list valuset;
      Data: list valuset
      }.
   Definition file_rep:= list file.
   
-  Definition rep (fr: file_rep) := arrayN  (@ptsto addr _ _) 0 fr.
+  Definition rep (fr: file_rep) := (arrayN  (@ptsto addr _ _) 0 fr * [[ forall f, In f fr -> length (Data f) = file_size ]])%pred.
   
   Definition upd_file (fr: file_rep) fn bn vs fdef:= 
           let file :=  (selN fr fn fdef) in
-          updN fr fn  {| 
-                                Meta:= Meta file;
-                                Data:= (updN (Data file) bn vs)
-                            |}.
+          updN fr fn  {| Data:= (updN (Data file) bn vs) |}.
 
-  Definition read_from_file arr (fr: file_rep) fn bn vsdef:=
+  Definition read_from_file arr (fr: file_rep) fn bn fdef vsdef:=
     if lt_dec fn (length fr) then
-      if lt_dec bn file_size then
+      let file := selN fr fn fdef in
+      if lt_dec bn (length (Data file)) then
         vs <- read_data arr (file_size * fn + bn) vsdef; 
         Ret (arr, vs)
       else
@@ -600,7 +1113,7 @@ Import L1.
   Definition write_to_file arr fr fn bn v fdef vsdef:=
     if lt_dec fn (length fr) then
       let file := selN fr fn fdef in
-      if lt_dec bn file_size then
+      if lt_dec bn (length (Data file)) then
         arr' <- write_data arr (file_size * fn + bn) v vsdef; 
         let vs := selN (Data file) bn vsdef in
         Ret (arr', upd_file fr fn bn (v, vsmerge vs) fdef)
@@ -609,8 +1122,183 @@ Import L1.
     else
       Ret (arr, fr).
   
+  Definition arr2file arr : (@mem addr addr_eq_dec file) :=
+  fun a => let fc := firstn file_size (skipn (file_size * a) (L1.Data arr)) in
+           match fc with
+           | nil => None
+           | _ => Some {| Data := fc |}
+           end.           
+
+  Definition equiv (pd: pred) (pu: pred) :=
+   forall md arr,
+      L1.rep arr md
+      -> pd md
+      -> pu (arr2file arr).
+      
+      
+  Inductive prog_secure T (p: prog T) pre post :=
+  | STD :
+      prog_secure_strict p pre post
+      -> prog_secure p pre post
+  | REL : forall pre' post',
+      equiv pre' pre
+      -> equiv post' post
+      -> prog_secure_strict p pre' post'
+      -> prog_secure p pre post.
+            
 End L2.
 
+Lemma ret_secure_strict_frame : forall T AT AEQ V (v: T) (F: @pred AT AEQ V) ,
+    prog_secure_strict (Ret v) F F.
+Proof.
+  intros; eapply PSImpl.
+  3: eapply PSFrame.
+  3: eauto.
+  cancel.
+  cancel.
+Qed.
+
+Lemma ret_secure_strict_frame_pimpl : forall T AT AEQ V (v: T) (F F': @pred AT AEQ V) ,
+    F =p=> F' ->
+    prog_secure_strict (Ret v) F F'.
+Proof.
+  intros; eapply PSImpl.
+  3: eapply PSFrame.
+  3: eauto.
+  cancel.
+  cancel.
+Qed.
+
+Hint Resolve ret_secure_strict_frame.
+Hint Resolve ret_secure_strict_frame_pimpl.
+
+Theorem read_data_secure_strict:
+  forall V arr i (v: V) def,
+  @prog_secure_strict _ _ addr_eq_dec _ (L1.read_data arr i def) (i|-> v) (i|-> v).
+Proof.
+  intros.
+  unfold L1.read_data.
+  destruct (lt_dec i (length (L1.Data arr))); eauto.
+Qed.
+
+Theorem write_data_secure_strict:
+  forall arr i v vs def,
+  @prog_secure_strict _ _ addr_eq_dec _ (L1.write_data arr i v def)(i|-> vs) (i|-> vs \/ i|-> (v, vsmerge vs)).
+Proof.
+  intros.
+  unfold L1.write_data.
+  destruct (lt_dec i (length (L1.Data arr))); eauto.
+  econstructor; eauto.
+  intros; apply ret_secure_strict_frame_pimpl; cancel.
+  apply ret_secure_strict_frame_pimpl; cancel.
+Qed.
+
+Hint Resolve read_data_secure_strict.
+Hint Resolve write_data_secure_strict.
+
+
+Theorem read_from_file_secure_strict:
+  forall arr fr fn bn fdef vsdef (f: L2.file) Ff,
+      L2.rep fr (L2.arr2file arr)
+      -> (Ff * fn |-> f)%pred (list2nmem fr)
+      -> L2.prog_secure (L2.read_from_file arr fr fn bn fdef vsdef) (fn|-> f)%pred (fn|-> f)%pred.
+Proof.
+    intros.
+    unfold L2.rep in *.
+    (* apply list2nmem_array_mem_eq in H0; subst.
+    rewrite <- H0 in H. *)
+
+    unfold L2.read_from_file.
+    destruct (lt_dec fn (length fr)); try solve [econstructor; eauto].
+    destruct (lt_dec bn (length (L2.Data fr ⟦ fn ⟧))); try solve [econstructor; eauto].
+    
+    eapply L2.REL.
+    
+    - instantiate (1:= arrayN (ptsto (V:=valuset)) (L2.file_size * fn) (L2.Data f)).
+    
+    unfold L2.equiv, L1.rep, L2.rep; intros m arr' Hr1 Hu.
+    apply list2nmem_array_mem_eq in Hr1; subst.
+    destruct_lift H.
+    apply emp_star; apply sep_star_comm; apply mem_except_ptsto.
+    unfold L2.arr2file.
+    destruct (firstn L2.file_size (skipn (L2.file_size * fn) (L1.Data arr'))) eqn:D.
+     + apply length_zero_iff_nil in D.
+       rewrite firstn_length in D.
+       destruct (lt_dec (length (skipn (L2.file_size * fn) (L1.Data arr'))) L2.file_size).
+       * rewrite min_r in D; try omega.
+         assert (A: (skipn (L2.file_size * fn) (L1.Data arr') = nil)).
+         apply length_zero_iff_nil; auto.
+         apply emp_star in Hu; apply arrayN_list2nmem in Hu.
+         rewrite A in *; simpl in *.
+         rewrite firstn_nil in Hu.
+         eapply list2nmem_sel in H0; subst.
+         rewrite H0 in *.
+         apply length_zero_iff_nil in Hu; rewrite Hu in *; omega.
+         repeat constructor; assumption.
+       * rewrite min_l in D; try omega.
+         exfalso; apply L2.file_size_nonzero; auto.
+     + rewrite <- D in *.
+       apply emp_star in Hu; eapply arrayN_list2nmem in Hu.
+       destruct_lift H.
+       specialize (H3 f).
+       rewrite H3 in Hu.
+       rewrite <- Hu; destruct f; simpl; auto.
+       eapply in_selN in l.
+       eapply list2nmem_sel in H0; subst.
+       rewrite H0 in *; eauto.
+       repeat constructor; assumption.
+     + unfold emp; intros.
+       destruct (addr_eq_dec fn a); subst.
+       apply mem_except_eq.
+       rewrite mem_except_ne; auto.
+       assert (list2nmem (list2nmem (L1.Data arr')))
+       destruct (lt_dec a fn).
+       
+       unfold L2.arr2file.
+       destruct (firstn L2.file_size (skipn (L2.file_size * a) (L1.Data arr'))) eqn:D; auto.
+         + apply length_zero_iff_nil in D.
+           rewrite firstn_length in D.
+           destruct (lt_dec (length (skipn (L2.file_size * fn) (L1.Data arr'))) L2.file_size).
+           * rewrite min_r in D; try omega.
+             assert (A: (skipn (L2.file_size * fn) (L1.Data arr') = nil)).
+             apply length_zero_iff_nil; auto.
+             apply emp_star in Hu; apply arrayN_list2nmem in Hu.
+             rewrite A in *; simpl in *.
+             rewrite firstn_nil in Hu.
+             eapply list2nmem_sel in H0; subst.
+             rewrite H0 in *.
+             apply length_zero_iff_nil in Hu; rewrite Hu in *; omega.
+             repeat constructor; assumption.
+           * rewrite min_l in D; try omega.
+             exfalso; apply L2.file_size_nonzero; auto.
+       
+     unfold L2.arr2file.
+       destruct (firstn L2.file_size (skipn (L2.file_size * a') (L1.Data arr'))) eqn:D; auto.
+       eapply nth_error_In.
+       Search nth_error.
+       apply ptsto_valid' in H0.
+       unfold nth_error, list2nmem in *.
+       Search list2nmem selN.
+    Locate "|->?".
+    Search exis ptsto.
+    eexists; eapply list2nmem_array_exis.
+    Search arrayN_ex ptsto.
+    apply list2nmem_array_pick.
+    rewrite <- Hr2 in Hu; clear Hr2.
+    destruct Hu.
+    unfold L2.arr2file in *; simpl in *.
+    destruct (firstn L2.file_size (skipn (L2.file_size * fn) (L1.Data arr'))) eqn:D.
+    inversion H1.
+    eapply list2nmem_sel_inb.
+
+    eapply L2.REL; [ | | econstructor; eauto].
+    
+    econstructor.
+    unfold list2nmem.
+    erewrite selN_map.
+    Search selN length.
+    destruct (firstn L2.file_size (skipn (L2.file_size * a) (L1.Data arr0))) eqn:D.
+Admitted.
 
 Theorem read_log_secure:
   forall arr i v def,
@@ -667,90 +1355,6 @@ Qed.
 
 
 
-Module NewDef.
-Inductive prog_secure_strict: forall T AT AEQ V, prog T -> @pred AT AEQ V -> @pred AT AEQ V -> Prop :=
-| PSRet : forall T AT AEQ V (v: T), 
-      @prog_secure_strict T AT AEQ V (Ret v) emp emp
-| PSRead : forall V a (vs: V),
-      @prog_secure_strict _ _ addr_eq_dec _ (Read a) (a|->vs) (a|->vs)
-| PSWrite : forall a v vs,
-      @prog_secure_strict _ _ addr_eq_dec _ (Write a v) (a |-> vs)%pred (a |-> (v, vsmerge vs))%pred
-| PSBind : forall AT AEQ V T1 T2 (p1 : prog T1) (p2 : T1 -> prog T2) (pre post1 post2: @pred AT AEQ V),
-      prog_secure_strict p1 pre post1 ->
-      (forall x, prog_secure_strict (p2 x) post1 post2) ->
-      prog_secure_strict (Bind p1 p2) pre post2
-| PSImpl : forall T AT AEQ V (p : prog T) (pre pre' post post': @pred AT AEQ V),
-      pre' =p=> pre ->
-      post =p=> post' ->
-      prog_secure_strict p pre post ->
-      prog_secure_strict p pre' post'
-| PSFrame : forall T AT AEQ V (p : prog T) (pre post F: @pred AT AEQ V),
-  prog_secure_strict p pre post ->
-  prog_secure_strict p (F * pre)%pred (F * post)%pred.
-
-Hint Constructors prog_secure_strict.
-
-Lemma ret_secure_strict_frame : forall T AT AEQ V (v: T) (F: @pred AT AEQ V) ,
-    prog_secure_strict (Ret v) F F.
-Proof.
-  intros; eapply PSImpl.
-  3: eapply PSFrame.
-  3: eauto.
-  cancel.
-  cancel.
-Qed.
-
-Lemma ret_secure_strict_frame_pimpl : forall T AT AEQ V (v: T) (F F': @pred AT AEQ V) ,
-    F =p=> F' ->
-    prog_secure_strict (Ret v) F F'.
-Proof.
-  intros; eapply PSImpl.
-  3: eapply PSFrame.
-  3: eauto.
-  cancel.
-  cancel.
-Qed.
-
-Hint Resolve ret_secure_strict_frame.
-Hint Resolve ret_secure_strict_frame_pimpl.
-
-Theorem read_data_secure_strict:
-  forall V arr i (v: V) def,
-  @prog_secure_strict _ _ addr_eq_dec _ (L1.read_data arr i def)((i+length(L1.Log arr))|-> v) ((i+length(L1.Log arr))|-> v).
-Proof.
-  intros.
-  unfold L1.read_data.
-  destruct (lt_dec i (length (L1.Data arr))); eauto.
-Qed.
-
-Theorem write_data_secure_strict:
-  forall arr i v vs def,
-  @prog_secure_strict _ _ addr_eq_dec _ (L1.write_data arr i v def)((i+length(L1.Log arr))|-> vs) ((i+length(L1.Log arr))|-> vs \/ (i+length(L1.Log arr))|-> (v, vsmerge vs)).
-Proof.
-  intros.
-  unfold L1.write_data.
-  destruct (lt_dec i (length (L1.Data arr))); eauto.
-  econstructor; eauto.
-  intros; apply ret_secure_strict_frame_pimpl; cancel.
-  apply ret_secure_strict_frame_pimpl; cancel.
-Qed.
-
-Hint Resolve read_data_secure_strict.
-Hint Resolve write_data_secure_strict.
-
-
-Theorem read_from_file_secure_strict:
-  forall arr fr fn bn vsdef (f: L2.file),
-      @prog_secure_strict _ _ addr_eq_dec _ (L2.read_from_file arr fr fn bn vsdef) (fn|-> f) (fn|-> f).
-Proof.
-    intros.
-    unfold L2.read_from_file.
-    destruct (lt_dec fn (length fr)); eauto.
-    destruct (lt_dec bn L2.file_size); eauto.
-    econstructor; eauto.
-Admitted.
-
-End NewDef.
 
 
 End TwoLevel.
