src/DirMem.v
@@ -1,0 +1,54 @@
+Require Import Mem.
+Require Import DirTreeDef.
+Require Import String.
+Require Import List.
+Require Import Pred.
+
+Set Implicit Parameters.
+
+Definition addr := nat.
+
+Inductive dirtree_node:=
+  | DtnFile : addr -> dirfile -> dirtree_node
+  | DtnDir  : addr -> list string -> dirtree_node.
+
+Definition splitter {A B C} (f: A -> B -> C) (v: A * B):= f (fst v) (snd v).
+
+Definition extend_path (path: list string) (pt: string * dirtree):=
+  ((path++(fst pt)::nil)%list, snd pt).
+
+Fixpoint depth (d: dirtree) : nat.
+  induction d.
+  apply 1.
+  apply (1 + fold_left max (map depth (snd (split l))) 0).
+Qed.
+
+(* Fixpoint depth (d: dirtree) :=
+  match d with
+  | TreeFile _ _ => 1
+  | TreeDir _ dirs => 1 + fold_left max (map depth (snd (split dirs))) 0
+  end. *)
+
+
+Fixpoint dir2mem' (depth: nat) (path: list string) (tree: dirtree) : @mem (list string) (list_eq_dec string_dec) dirfile :=
+ match depth with
+ | O => empty_mem
+ | S d' =>
+     match tree with 
+     | TreeFile _ f => insert empty_mem path f
+     | TreeDir _ dirs => fold_left (@mem_union (list string) (list_eq_dec string_dec) dirfile)
+                          (map (splitter (dir2mem' d'))
+                              (map (extend_path path) dirs)) empty_mem
+     end
+ end.
+   
+
+Definition dir2mem d := dir2mem' (Depth d) nil d.
+
+
+
+Fixpoint mem_union_list {AT AEQ V} (m: @mem AT AEQ V) ml :=
+match ml with
+| nil => m
+| h::t => mem_union_list (mem_union m h) t
+end.
