src/Prog2.v
@@ -1,0 +1,253 @@
+Require Import FunctionalExtensionality.
+Require Import Structures.OrderedType.
+Require Import Structures.OrderedTypeEx.
+Require Import Omega.
+Require Import List.
+Require Import Mem.
+Require Import PredCrash.
+Require Import AsyncDisk.
+Require Import Word.
+Require Import String.
+
+Import ListNotations.
+
+Set Implicit Arguments.
+
+(** * The programming language *)
+
+Parameter vartype : Type.
+Parameter vartype_eq_dec : forall (x y : vartype), {x=y}+{x<>y}.
+
+Polymorphic Inductive var_value : Type :=
+  | Any : forall (T : Type), T -> var_value.
+
+Inductive mem_prog : Type -> Type :=
+  | Read (a: addr) : mem_prog valu
+  | Write (a: addr) (v: valu) : mem_prog unit
+  | Trim (a: addr) : mem_prog unit.
+
+Inductive var_prog : Type -> Type :=
+  | VarAlloc (T : Type) (v : T) : var_prog vartype
+  | VarDelete (i : vartype) : var_prog unit
+  | VarGet (i : vartype) (T : Type) : var_prog T
+  | VarSet (i : vartype) (T : Type) (v : T) : var_prog unit.
+
+Arguments VarAlloc {T} v.
+Arguments VarGet i {T}.
+Arguments VarSet i {T} v.
+
+
+(** single program *)
+Inductive prog : Type -> Type :=
+  | Ret T (v: T) : prog T
+  | Mem T (p: @mem_prog T) : prog T
+  | Var T (p: @var_prog T) : prog T
+  | Sync : prog unit
+  | AlertModified : prog unit
+  | Debug (s: string) (n: nat) : prog unit
+  | Rdtsc: prog nat
+  | Hash (sz: nat) (buf: word sz) : prog (word hashlen)
+  | Hash2 (sz1 sz2: nat) (buf1 : word sz1) (buf2 : word sz2) : prog (word hashlen)
+  | Bind T T' (p1: prog T) (p2: T -> prog T') : prog T'.
+
+Arguments Ret {T} v.
+Arguments Mem {T} p.
+Arguments Var {T} p.
+
+
+Definition varmem := @mem vartype vartype_eq_dec var_value.
+
+Inductive outcome (T : Type) :=
+  | Failed
+  | Finished (m: rawdisk) (v: varmem) (hm: hashmap) (v: T)
+  | Crashed (m: rawdisk) (hm: hashmap).
+  
+Inductive mem_step : forall T,
+    rawdisk -> varmem -> hashmap -> mem_prog T ->
+    rawdisk -> varmem -> hashmap -> T -> Prop :=
+    
+| StepRead : forall m a v x vm hm,
+    m a = Some (v, x) ->
+    mem_step m vm hm (Read a) m vm hm v
+| StepWrite : forall m a v v0 x vm hm,
+    m a = Some (v0, x) ->
+    mem_step m vm hm (Write a v) (upd m a (v, v0 :: x)) vm hm tt
+| StepTrim : forall m a vs vs' vm hm,
+    m a = Some vs ->
+    mem_step m vm hm (Trim a) (upd m a vs') vm hm tt.
+
+
+Inductive var_step : forall T,
+    rawdisk -> varmem -> hashmap -> var_prog T ->
+    rawdisk -> varmem -> hashmap -> T -> Prop :=
+    
+| StepVarAlloc : forall T d v vm i hm,
+    vm i = None ->
+    var_step d vm hm (@VarAlloc T v) d (insert vm i (@Any T v)) hm i
+| StepVarDelete : forall d v vm i hm,
+    vm i = Some v ->
+    var_step d vm hm (VarDelete i) d (delete vm i) hm tt
+| StepVarGet : forall T d v vm i hm,
+    vm i = Some (@Any T v) ->
+    var_step d vm hm (@VarGet i T) d vm hm v
+| StepVarSet : forall T d v0 v vm i hm,
+    vm i = Some v0 ->
+    var_step d vm hm (@VarSet i T v) d (upd vm i (@Any T v)) hm tt.
+
+Inductive step : forall T,
+    rawdisk -> varmem -> hashmap -> prog T ->
+    rawdisk -> varmem -> hashmap -> T -> Prop :=
+| StepMem : forall T m vm hm (p: mem_prog T) m' r,
+    mem_step m vm hm p m' vm hm r ->
+    step m vm hm (Mem p) m' vm hm r
+| StepVar : forall T m vm hm (p: var_prog T) vm' r,
+    var_step m vm hm p m vm' hm r ->
+    step m vm hm (Var p) m vm' hm r
+| StepSync : forall m vm hm,
+    step m vm hm (Sync) (sync_mem m) vm hm tt
+| StepHash : forall m sz (buf : word sz) h vm hm,
+    hash_safe hm h buf ->
+    hash_fwd buf = h ->
+    step m vm hm (Hash buf) m vm (upd_hashmap' hm h buf) h
+| StepHash2 : forall m sz1 sz2 (buf1 : word sz1) (buf2 : word sz2) (buf : word (sz1 + sz2)) h vm hm,
+    buf = Word.combine buf1 buf2 ->
+    hash_safe hm h buf ->
+    hash_fwd buf = h ->
+    step m vm hm (Hash2 buf1 buf2) m vm (upd_hashmap' hm h buf) h.
+    
+    
+Inductive fail_mem_step : forall T,
+    rawdisk -> varmem -> mem_prog T -> Prop :=
+| FailRead : forall m vm a,
+    m a = None ->
+    fail_mem_step m vm (Read a)
+| FailWrite : forall m vm a v,
+    m a = None ->
+    fail_mem_step m vm (Write a v)
+| FailTrim : forall m vm a,
+    m a = None ->
+    fail_mem_step m vm (Trim a).
+    
+Inductive fail_var_step : forall T,
+    rawdisk -> varmem -> var_prog T -> Prop :=
+| FailVarDelete : forall m vm i,
+    vm i = None ->
+    fail_var_step m vm (VarDelete i)
+| FailVarGetType : forall T T' m vm i (v : T'),
+    T <> T' ->
+    vm i = Some (Any v) ->
+    fail_var_step m vm (@VarGet i T)
+| FailVarGetNone : forall T m vm i,
+    vm i = None ->
+    fail_var_step m vm (@VarGet i T)
+| FailVarSetNone : forall T m vm i (v : T),
+    vm i = None ->
+    fail_var_step m vm (VarSet i v).
+
+
+Inductive fail_step : forall T,
+    rawdisk -> varmem -> prog T -> Prop :=
+| FailMem : forall T m vm (p: mem_prog T),
+    fail_mem_step m vm p ->
+    fail_step m vm (Mem p)
+| FailVar : forall T m vm (p: var_prog T),
+    fail_var_step m vm p ->
+    fail_step m vm (Var p).
+
+Inductive crash_mem_step : forall T, mem_prog T -> Prop :=
+| CrashRead : forall a,
+    crash_mem_step (Read a)
+| CrashWrite : forall a v,
+    crash_mem_step (Write a v).
+    
+    
+Inductive crash_step : forall T, prog T -> Prop :=
+| MemCrash : forall T (p: mem_prog T),
+    crash_mem_step p ->
+    crash_step (Mem p).
+
+Inductive exec : forall T, rawdisk -> varmem -> hashmap -> prog T -> outcome T -> Prop :=
+| XRet : forall T m vm hm (v: T),
+    exec m vm hm (Ret v) (Finished m vm hm v)
+| XAlertModified : forall m vm hm,
+    exec m vm hm (AlertModified) (Finished m vm hm tt)
+| XDebug : forall m vm hm s a,
+    exec m vm hm (Debug s a) (Finished m vm hm tt)
+| XRdtsc : forall m vm hm t,
+    exec m vm hm (Rdtsc) (Finished m vm hm t)
+| XStep : forall T m vm hm (p: prog T) m' vm' hm' v,
+    step m vm hm p m' vm' hm' v ->
+    exec m vm hm p (Finished m' vm' hm' v)
+| XBindFinish : forall m vm hm T (p1: prog T) m' vm' hm' (v: T)
+                  T' (p2: T -> prog T') out,
+    exec m vm hm p1 (Finished m' vm' hm' v) ->
+    exec m' vm' hm' (p2 v) out ->
+    exec m vm hm (Bind p1 p2) out
+| XBindFail : forall m vm hm T (p1: prog T)
+                T' (p2: T -> prog T'),
+    exec m vm hm p1 (Failed T) ->
+    exec m vm hm (Bind p1 p2) (Failed T')
+| XBindCrash : forall m vm hm T (p1: prog T) m' hm'
+                 T' (p2: T -> prog T'),
+    exec m vm hm p1 (Crashed T m' hm') ->
+    exec m vm hm (Bind p1 p2) (Crashed T' m' hm')
+| XFail : forall m vm hm T (p: prog T),
+    fail_step m vm p ->
+    exec m vm hm p (Failed T)
+| XCrash : forall m vm hm T (p: prog T),
+    crash_step p ->
+    exec m vm hm p (Crashed T m hm).
+
+(** program with recovery *)
+Inductive recover_outcome (TF TR: Type) :=
+  | RFailed
+  | RFinished (m: rawdisk) (vm: varmem) (hm: hashmap) (v: TF)
+  | RRecovered (m: rawdisk) (vm: varmem) (hm: hashmap) (v: TR).
+
+Inductive exec_recover (TF TR: Type)
+    : rawdisk -> varmem -> hashmap -> prog TF -> prog TR -> recover_outcome TF TR -> Prop :=
+  | XRFail : forall m vm hm p1 p2, exec m vm hm p1 (Failed TF)
+    -> exec_recover m vm hm p1 p2 (RFailed TF TR)
+  | XRFinished : forall m vm hm p1 p2 m' vm' hm' (v: TF), exec m vm hm p1 (Finished m' vm' hm' v)
+    -> exec_recover m vm hm p1 p2 (RFinished TR m' vm' hm' v)
+  | XRCrashedFailed : forall m vm hm p1 p2 m' hm' m'r, exec m vm hm p1 (Crashed TF m' hm')
+    -> possible_crash m' m'r
+    -> @exec_recover TR TR m'r empty_mem hm' p2 p2 (RFailed TR TR)
+    -> exec_recover m vm hm p1 p2 (RFailed TF TR)
+  | XRCrashedFinished : forall m vm hm p1 p2 m' hm' m'r m'' vm'' hm'' (v: TR), exec m vm hm p1 (Crashed TF m' hm')
+    -> possible_crash m' m'r
+    -> @exec_recover TR TR m'r empty_mem hm' p2 p2 (RFinished TR m'' vm'' hm'' v)
+    -> exec_recover m vm hm p1 p2 (RRecovered TF m'' vm'' hm'' v)
+  | XRCrashedRecovered : forall m vm hm p1 p2 m' hm' m'r m'' vm'' hm'' (v: TR), exec m vm hm p1 (Crashed TF m' hm')
+    -> possible_crash m' m'r
+    -> @exec_recover TR TR m'r empty_mem hm' p2 p2 (RRecovered TR m'' vm'' hm'' v)
+    -> exec_recover m vm hm p1 p2 (RRecovered TF m'' vm'' hm'' v).
+
+Hint Constructors exec.
+Hint Constructors step.
+Hint Constructors exec_recover.
+
+(** program notations *)
+
+Definition pair_args_helper (A B C:Type) (f: A->B->C) (x: A*B) := f (fst x) (snd x).
+Notation "^( a )" := (pair a tt).
+Notation "^( a , .. , b )" := (pair a .. (pair b tt) .. ).
+
+Notation "p1 ;; p2" := (Bind p1 (fun _: unit => p2)) (at level 60, right associativity).
+Notation "x <- p1 ; p2" := (Bind p1 (fun x => p2)) (at level 60, right associativity,
+                                                 format "'[v' x  <-  p1 ; '/' p2 ']'").
+Notation "'let^' ( a ) <- p1 ; p2" :=
+  (Bind p1
+    (pair_args_helper (fun a (_:unit) => p2))
+  )
+  (at level 60, right associativity, a ident,
+   format "'[v' let^ ( a )  <-  p1 ; '/' p2 ']'").
+
+Notation "'let^' ( a , .. , b ) <- p1 ; p2" :=
+  (Bind p1
+    (pair_args_helper (fun a => ..
+      (pair_args_helper (fun b (_:unit) => p2))
+    ..))
+  )
+    (at level 60, right associativity, a closed binder, b closed binder,
+     format "'[v' let^ ( a , .. , b )  <-  p1 ; '/' p2 ']'").
